typed_instr and typed_body need the heap_ctx; prove assignment (based on typed_writing)

theories/typing/programs.v
@@ -8,9 +8,10 @@ Section typing.
   Context `{typeG Σ}.
 
   (** Function Body *)
+  (* This is an iProp because it is also used by the function type. *)
   Definition typed_body (E : elctx) (L : llctx) (C : cctx) (T : tctx)
                         (e : expr) : iProp Σ :=
-    (∀ tid qE, lft_ctx -∗ elctx_interp E qE -∗ llctx_interp L 1 -∗
+    (∀ tid qE, heap_ctx -∗ lft_ctx -∗ elctx_interp E qE -∗ llctx_interp L 1 -∗
                (elctx_interp E qE -∗ cctx_interp tid C) -∗ tctx_interp tid T -∗
                WP e {{ _, cont_postcondition }})%I.
   Global Arguments typed_body _ _ _ _ _%E.
@@ -31,25 +32,26 @@ Section typing.
     Proper (flip (cctx_incl E) ==> flip (tctx_incl E L) ==> eq ==> (⊢)) (typed_body E L).
   Proof.
     intros C1 C2 HC T1 T2 HT e ? <-. iIntros "H".
-    iIntros (tid qE) "#LFT HE HL HC HT".
+    iIntros (tid qE) "#HEAP #LFT HE HL HC HT".
     iMod (HT with "LFT HE HL HT") as "(HE & HL & HT)".
-    iApply ("H" with "LFT HE HL [HC] HT").
+    iApply ("H" with "HEAP LFT HE HL [HC] HT").
     iIntros "HE". by iApply (HC with "LFT HC").
   Qed.
 
   (** Instruction *)
   Definition typed_instruction (E : elctx) (L : llctx)
-             (T1 : tctx) (e : expr) (T2 : val → tctx) : iProp Σ :=
-    (∀ tid qE, □ (lft_ctx -∗ elctx_interp E qE -∗ llctx_interp L 1 -∗ tctx_interp tid T1 -∗
-                   WP e {{ v, elctx_interp E qE ∗ llctx_interp L 1 ∗ tctx_interp tid (T2 v) }}))%I.
+             (T1 : tctx) (e : expr) (T2 : val → tctx) : Prop :=
+    ∀ tid qE, heap_ctx -∗ lft_ctx -∗ elctx_interp E qE -∗ llctx_interp L 1 -∗ tctx_interp tid T1 -∗
+                   WP e {{ v, elctx_interp E qE ∗ llctx_interp L 1 ∗ tctx_interp tid (T2 v) }}.
   Global Arguments typed_instruction _ _ _ _%E _.
 
   (** Writing and Reading **)
   Definition typed_writing (E : elctx) (L : llctx) (ty1 ty ty2 : type) : Prop :=
-    ∀ v tid E, lftE ∪ (↑lrustN) ⊆ E →
-      lft_ctx -∗ ty1.(ty_own) tid [v] ={E}=∗
-        ∃ l vl, ⌜length vl = ty.(ty_size)⌝ ∗ l ↦∗ vl ∗
-        ∀ vl', l ↦∗ vl' -∗ ▷ (ty.(ty_own) tid vl') ={E}=∗ ty2.(ty_own) tid [v].
+    ∀ v tid F qE qL, lftE ∪ (↑lrustN) ⊆ F →
+      lft_ctx -∗ elctx_interp E qE -∗ llctx_interp L qL -∗ ty1.(ty_own) tid [v] ={F}=∗
+        ∃ (l : loc) vl, ⌜length vl = ty.(ty_size) ∧ v = #l⌝ ∗ l ↦∗ vl ∗
+        ∀ vl', l ↦∗ vl' -∗ (ty.(ty_own) tid vl') ={F}=∗
+                  elctx_interp E qE ∗ llctx_interp L qL ∗ ty2.(ty_own) tid [v].
 End typing.
 
 Notation typed_instruction_ty E L T1 e ty := (typed_instruction E L T1 e (λ v : val, [TCtx_hasty v ty])).
@@ -63,10 +65,30 @@ Section typing_rules.
     (∀ v : val, typed_body E L C (T2 v ++ T) (subst' xb v e')) →
     typed_body E L C (T1 ++ T) (let: xb := e in e').
   Proof.
-    iIntros (Hc He He' tid qE) "#LFT HE HL HC HT". rewrite tctx_interp_app.
+    iIntros (Hc He He' tid qE) "#HEAP #LFT HE HL HC HT". rewrite tctx_interp_app.
     iDestruct "HT" as "[HT1 HT]". wp_bind e. iApply (wp_wand with "[HE HL HT1]").
-    { iApply (He with "LFT HE HL HT1"). }
+    { iApply (He with "HEAP LFT HE HL HT1"). }
     iIntros (v) "/= (HE & HL & HT2)". iApply wp_let; first wp_done. iModIntro.
-    iApply (He' with "LFT HE HL HC [HT2 HT]"). rewrite tctx_interp_app. by iFrame.
+    iApply (He' with "HEAP LFT HE HL HC [HT2 HT]"). rewrite tctx_interp_app. by iFrame.
   Qed.
+  
+  Lemma type_assign E L ty1 ty ty1' p1 p2 :
+    typed_writing E L ty1 ty ty1' →
+    typed_instruction E L [TCtx_hasty p1 ty1; TCtx_hasty p2 ty] (p1 <- p2)
+                      (λ _, [TCtx_hasty p1 ty1']).
+  Proof.
+    iIntros (Hwrt tid qE) "#HEAP #LFT HE HL".
+    rewrite tctx_interp_cons tctx_interp_singleton. iIntros "[Hp1 Hp2]".
+    wp_bind p1. iApply (wp_hasty with "Hp1"). iIntros (v1) "% Hown1".
+    wp_bind p2. iApply (wp_hasty with "Hp2"). iIntros (v2) "_ Hown2".
+    iMod (Hwrt with "* LFT HE HL Hown1") as (l vl) "([% %] & Hl & Hclose)"; first done.
+    subst v1. iAssert (⌜1%nat = ty_size ty⌝%I) with "[#]" as %Hsz.
+    { change (1%nat) with (length [v2]). by iApply ty_size_eq. }
+    rewrite <-Hsz in *. destruct vl as [|v[|]]; try done.
+    rewrite heap_mapsto_vec_singleton. wp_write.
+    rewrite -heap_mapsto_vec_singleton.
+    iMod ("Hclose" with "* Hl Hown2") as "($ & $ & Hown)".
+    rewrite tctx_interp_singleton tctx_hasty_val' //.
+  Qed.
+
 End typing_rules.
